33

HumanEvalLean/HumanEval33.lean
@@ -1,7 +1,114 @@
 module
 
-def sort_third : Unit :=
-  ()
+public import Std
+import all Init.Data.Range.Polymorphic.UpwardEnumerable -- UpwardEnumerable.least not exposed
+open Std Std.Iterators Std.Iterators.Types Std.Do
+
+set_option mvcgen.warning false
+
+/-! ## Implementation -/
+
+public section
+
+-- TODO: use `Array.mergeSort` when available
+
+def sortThird (xs : Array Int) : Array Int := Id.run do
+  let sorted := xs.iter.stepSize 3 |>.toList.mergeSort.toArray
+  -- Prove the size of `sorted` so that we can access `sorted[i]` without a runtime bounds check
+  have : sorted.size = (xs.size + 2) / 3 := by simp [sorted, Iter.length_stepSize]
+  let mut vec := xs.toVector
+  for h : i in *...((xs.size + 2) / 3) do
+    vec := vec.set (i * 3) sorted[i]
+  return vec.toArray
+
+/-! ## Tests -/
+
+example : sortThird #[1, 2, 3] = #[1, 2, 3] := by native_decide
+example : sortThird #[5, 3, -5, 2, -3, 3, 9, 0, 123, 1, -10] =
+    #[1, 3, -5, 2, -3, 3, 5, 0, 123, 9, -10] := by native_decide
+example : sortThird #[5, 8, -12, 4, 23, 2, 3, 11, 12, -10] =
+    #[-10, 8, -12, 3, 23, 2, 4, 11, 12, 5] := by native_decide
+example : sortThird #[5, 6, 3, 4, 8, 9, 2] = #[2, 6, 3, 4, 8, 9, 5] := by native_decide
+example : sortThird #[5, 8, 3, 4, 6, 9, 2] = #[2, 8, 3, 4, 6, 9, 5] := by native_decide
+example : sortThird #[5, 6, 9, 4, 8, 3, 2] = #[2, 6, 9, 4, 8, 3, 5] := by native_decide
+example : sortThird #[5, 6, 3, 4, 8, 9, 2, 1] = #[2, 6, 3, 4, 8, 9, 5, 1] := by native_decide
+
+/-! ## Missing API -/
+
+theorem Nat.eq_add_of_toList_rco_eq_append_cons {a b : Nat} {pref cur suff}
+    (h : (a...b).toList = pref ++ cur :: suff) :
+    cur = a + pref.length := by
+  have := Rco.eq_succMany?_of_toList_eq_append_cons h
+  simpa [PRange.UpwardEnumerable.least, PRange.least?] using this
+
+/-! ## Verification -/
+
+theorem getElem?_sortThird_of_mod_ne_zero {xs : Array Int} {i : Nat} (h : i % 3 ≠ 0) :
+    (sortThird xs)[i]? = xs[i]? := by
+  generalize hwp : sortThird xs = wp
+  apply Id.of_wp_run_eq hwp
+  mvcgen
+  invariants
+  · ⇓⟨cur, vec⟩ => ⌜∀ i : Nat, i % 3 ≠ 0 → vec[i]? = xs[i]?⌝
+  with grind [Vector.getElem?_mk]
+
+theorem getElem?_sortThird_mul_three {xs : Array Int} {i : Nat} :
+    (sortThird xs)[i * 3]? = (xs.iter.stepSize 3).toList.mergeSort[i]? := by
+  generalize hwp : sortThird xs = wp
+  apply Id.of_wp_run_eq hwp
+  mvcgen
+  invariants
+  · ⇓⟨cur, vec⟩ => ⌜∀ i < cur.pos, vec[i * 3]? = (xs.iter.stepSize 3).toList.mergeSort[i]?⌝
+  case vc1 =>
+    have := Nat.eq_add_of_toList_rco_eq_append_cons ‹_›
+    grind
+  case vc2 => grind
+  case vc3 => grind [Nat.length_toList_rio]
+
+/-!
+### Size properties
+
+The following two properties also follow from the two theorems above, but we provide them for
+good measure.
+-/
+
+theorem size_sortThird {xs : Array Int} :
+    (sortThird xs).size = xs.size := by
+  grind [sortThird]
+
+theorem length_stepSize {xs : Array Int} :
+    (xs.iter.stepSize 3).length = (xs.size + 2) / 3 := by
+  grind [Iter.length_stepSize]
+
+/-!
+### Correctness of used library functions
+
+For completeness, we point to library lemmas that prove the correctness of the `stepSize` and
+`List.mergeSort`, the library functions on which relied to state our formal lemmas.
+-/
+
+/--
+`(xs.iter.stepSize 3).toList` contains every element of `xs` at indices divisible by three,
+and no more elements than these.
+-/
+theorem getElem?_toList_stepSize {xs : Array Int} :
+    (xs.iter.stepSize 3).toList[i]? = xs[i * 3]? := by
+  grind [Iter.getElem?_toList_stepSize]
+
+/--
+info: List.mergeSort_perm.{u_1} {α : Type u_1} (l : List α) (le : α → α → Bool) : (l.mergeSort le).Perm l
+-/
+#guard_msgs in
+#check List.mergeSort_perm
+
+/--
+info: List.pairwise_mergeSort.{u_1} {α : Type u_1} {le : α → α → Bool}
+  (trans : ∀ (a b c : α), le a b = true → le b c = true → le a c = true)
+  (total : ∀ (a b : α), (le a b || le b a) = true) (l : List α) :
+  List.Pairwise (fun a b => le a b = true) (l.mergeSort le)
+-/
+#guard_msgs in
+#check List.pairwise_mergeSort
 
 /-!
 ## Prompt
